Begin fixing getchar correctness property (WIP)

progs/io_os_connection.v
@@ -7,7 +7,108 @@ Require Import compcert.lib.Integers.
 Require Import compcert.common.Memory.
 Require Import VST.progs.io_specs.
 Require Import VST.progs.io_dry.
+Require Import VST.floyd.sublist.
 Import ExtLib.Structures.Monad.
+
+Local Ltac inj :=
+  repeat match goal with
+  | H: _ = _ |- _ => assert_succeeds (injection H); inv H
+  end.
+
+Section CommonPrefix.
+
+  Context {A: Type}.
+  Variable Aeq : forall (x y : A), {x = y} + {x <> y}.
+
+  Fixpoint common_prefix (xs ys : list A) : list A :=
+    match xs, ys with
+    | x :: xs', y :: ys' =>
+      if Aeq x y then x :: common_prefix xs' ys' else nil
+    | _, _ => nil
+    end.
+
+  Definition split_at_common_prefix (xs ys : list A) : list A * list A :=
+    let i := length (common_prefix xs ys) in
+    let pre := firstn i xs in
+    let post := if length xs <=? length ys then skipn i ys else skipn i xs in
+    (pre, post).
+
+  Lemma common_prefix_sym : forall xs ys,
+    common_prefix xs ys = common_prefix ys xs.
+  Proof.
+    induction xs as [| x xs]; destruct ys as [| y ys]; cbn; auto.
+    destruct (Aeq x y), (Aeq y x); congruence.
+  Qed.
+
+  Lemma common_prefix_correct : forall xs ys,
+    let pre := common_prefix xs ys in
+    pre = firstn (length pre) xs.
+  Proof.
+    induction xs as [| x xs]; destruct ys as [| y ys]; cbn; auto.
+    destruct (Aeq x y); cbn; congruence.
+  Qed.
+
+  Lemma split_at_common_prefix_correct : forall xs ys,
+    length xs <= length ys ->
+    let (pre, post) := split_at_common_prefix xs ys in
+    ys = pre ++ post.
+  Proof.
+    induction xs as [| x xs]; destruct ys as [| y ys]; cbn; intros; auto; try lia.
+    rewrite leb_correct by lia.
+    destruct (Aeq x y); cbn; subst; auto.
+    rewrite <- common_prefix_correct.
+    rewrite common_prefix_sym.
+    rewrite common_prefix_correct at 1.
+    rewrite firstn_skipn.
+    auto.
+  Qed.
+
+  Fact list_eq_in_or : forall (xs ys xs' ys' : list A) x y,
+    xs ++ x :: xs' = ys ++ y :: ys' ->
+    x <> y ->
+    In y xs \/ In y xs'.
+  Proof.
+    induction xs; destruct ys; cbn; intros * Heq Hneq; inj; eauto.
+    - rewrite in_app_iff; cbn; auto.
+    - cut (In y xs \/ In y xs'); eauto.
+      intuition auto.
+  Qed.
+
+  Fact list_eq_in_l : forall (xs ys ys' : list A) x y,
+    xs ++ x :: nil = ys ++ y :: ys' ->
+    x <> y ->
+    In y xs.
+  Proof.
+    intros.
+    cut (In y xs \/ In y nil); [intuition |].
+    eapply list_eq_in_or; eauto.
+  Qed.
+
+  Fact list_eq_in_r : forall (xs' ys ys' : list A) x y,
+    x :: xs' = ys ++ y :: ys' ->
+    x <> y ->
+    In y xs'.
+  Proof.
+    intros.
+    cut (In y nil \/ In y xs'); [intuition |].
+    eapply list_eq_in_or; eauto.
+  Qed.
+
+  Fact list_unique_match : forall (xs ys xs' ys': list A) x,
+    xs ++ x :: xs' = ys ++ x :: ys' ->
+    NoDup (xs ++ x :: xs') ->
+    xs = ys /\ xs' = ys'.
+  Proof.
+    induction xs; destruct ys; cbn; intros * Heq Huniq; inj; inv Huniq; auto.
+    - rewrite in_app_iff in *; cbn in *.
+      intuition.
+    - rewrite in_app_iff in *; cbn in *.
+      intuition.
+    - cut (xs = ys /\ xs' = ys'); eauto.
+      intuition congruence.
+  Qed.
+
+End CommonPrefix.
 
 Import MonadNotation.
 Local Open Scope monad_scope.
@@ -36,29 +137,37 @@ Definition getchar_post' (m0 m : mem) r (witness : (int -> IO_itree) * IO_itree)
 
 (** Traces *)
 Inductive IO_trace_event :=
-| ETRead (r : Z)
+| ETReadOS (ridx : nat) (r : Z)
+| ETReadUser (ridx : nat) (r : Z)
 | ETWrite (c : Z).
 Definition etrace := list IO_trace_event.
 
+Definition IO_trace_event_eq (e1 e2 : IO_trace_event) : {e1 = e2} + {e1 <> e2} :=
+  ltac:(repeat decide equality).
+
 Definition trace_event_rtype (e : IO_trace_event) :=
   match e with
-  | ETRead _ => int
+  | ETReadOS _ _ => void
+  | ETReadUser _ _ => int
   | ETWrite _ => unit
   end.
 
 Definition io_event_of_io_tevent (e : IO_trace_event)
-  : IO_event (trace_event_rtype e) * (trace_event_rtype e) :=
+  : option (IO_event (trace_event_rtype e) * (trace_event_rtype e)) :=
   match e with
-  | ETRead r => (ERead, Int.repr r)
-  | ETWrite c => (EWrite (Int.repr c), tt)
+  | ETReadOS _ _ => None
+  | ETReadUser _ r => Some (ERead, Int.repr r)
+  | ETWrite c => Some (EWrite (Int.repr c), tt)
   end.
 
 Fixpoint trace_of_etrace (t : etrace) : @trace IO_event unit :=
   match t with
   | nil => TEnd
   | e :: t' =>
-      let (e', r) := io_event_of_io_tevent e in
-      TEventResponse e' r (trace_of_etrace t')
+      match io_event_of_io_tevent e with
+      | Some (e', r) => TEventResponse e' r (trace_of_etrace t')
+      | _ => trace_of_etrace t'
+      end
   end.
 
 Section SanityChecks.
@@ -89,7 +198,7 @@ Section SanityChecks.
     constructor.
   Qed.
 
-  Goal is_trace tree (trace_of_etrace (ETRead 0 :: nil)).
+  Goal is_trace tree (trace_of_etrace (ETReadUser O 0 :: ETReadOS O 0 :: nil)).
   Proof.
     hnf; cbn.
     repeat constructor.
@@ -114,109 +223,302 @@ Section Specs.
 
   Record state := mkSt {
     st_mem : mem;
-    st_console : list Z;
     st_trace : etrace;
   }.
+
+  Fixpoint compute_console (tr : etrace) : list (Z * nat) :=
+    match tr with
+    | nil => nil
+    | ev :: tr' =>
+        let cons := compute_console tr' in
+        match ev with
+        | ETReadOS ridx c =>
+            let cons' := if Zlength cons <? CONSOLE_MAX_LEN then cons
+                         else skipn 1 cons in
+            cons' ++ (c, ridx) :: nil
+        | ETReadUser _ _ => tl cons
+        | _ => cons
+        end
+    end.
 
   (* Read a character from the serial device and place it in the console buffer.
      Triggered by an interrupt from the serial device. *)
   Definition serial_getc (st : state) : state :=
-    let (mem, cons, tr) := st in
+    let (mem, tr) := st in
     let c := serial_oracle tr in
-    let cons' := if Zlength cons <? CONSOLE_MAX_LEN then cons
-                 else skipn 1 cons in
-    mkSt mem (cons' ++ c :: nil) (tr ++ ETRead c :: nil).
+    let ridx := length tr in
+    mkSt mem (ETReadOS ridx c :: tr).
 
   (* Take the first element from the console buffer or -1 if it is empty. *)
   Definition console_read (st : state) : state * Z :=
-    let (mem, cons, tr) := st in
-    match cons with
+    let (mem, tr) := st in
+    match compute_console tr with
     | nil => (st, -1)
-    | c :: rest =>
-      let st' := mkSt mem rest tr in
+    | (c, ridx) :: _ =>
+      let st' := mkSt mem (ETReadUser ridx c :: tr) in
       (st', c)
     end.
 
   (* Return the new state, the read character, and the section of the trace to
      be consumed. *)
-  Definition getchar_spec (st : state) : state * Z * etrace :=
+  Definition getchar_spec (st : state) : state * Z :=
     let (st', r) := console_read st in
     (* Success *)
-    if 0 <=? r then (st', r, ETRead r :: nil)
+    if 0 <=? r then (st', r)
     (* Error *)
-    else (st', -1, nil).
+    else (st', -1).
 
-  (* Invariant that everything in the trace was put there by the serial
-     device. *)
-  Definition valid_trace st :=
-    forall c,
-      In (ETRead c) st.(st_trace) ->
-      exists tr, serial_oracle tr = c.
+  (** Invariants *)
+  (* Everything in the trace was put there by the serial device. *)
+  Definition valid_trace_serial tr :=
+    forall ridx c,
+      In (ETReadOS ridx c) tr ->
+      exists tr',
+        serial_oracle tr' = c /\ length tr' = ridx /\
+        Zlength tr' <= Zlength tr /\
+        let lo := Z.max 0 (Zlength tr - (Zlength tr' + 1)) in
+        sublist lo (Zlength tr) tr = ETReadOS ridx c :: tr'.
 
-  (* Invariant that everything in the console buffer is also in the trace. *)
-  Definition valid_console st :=
-    Zlength st.(st_console) <= CONSOLE_MAX_LEN /\
-    forall c,
-      In c st.(st_console) ->
-      In (ETRead c) st.(st_trace).
+  (* Every user read has a matching OS read earlier in the trace. *)
+  Definition valid_trace_user tr :=
+    forall ridx c pre post,
+      tr = post ++ (ETReadUser ridx c) :: pre ->
+      In (ETReadOS ridx c) pre /\ hd_error (compute_console pre) = Some (c, ridx).
 
-  Definition valid_state st :=
-    valid_trace st /\ valid_console st.
+  (* Every event in the trace is unique. *)
+  Definition valid_trace_unique (tr : etrace) := NoDup tr.
 
-  Lemma serial_getc_preserve_valid_trace : forall st st',
-    valid_trace st ->
+  (* Everything in the console buffer is also in the trace. *)
+  Definition valid_console tr :=
+    forall ridx c,
+      In (c, ridx) (compute_console tr) ->
+      In (ETReadOS ridx c) tr.
+
+  (* The console buffer never overflows *)
+  Definition valid_console_len tr :=
+    Zlength (compute_console tr) <= CONSOLE_MAX_LEN.
+
+  Record valid_state st := {
+    valid_state_trace_serial : valid_trace_serial st.(st_trace);
+    (* Every user read has a matching OS read earlier in the trace. *)
+    valid_state_trace_user : valid_trace_user st.(st_trace);
+    (* Every event in the trace is unique. *)
+    valid_state_trace_unique : valid_trace_unique st.(st_trace);
+    (* Everything in the console buffer is also in the trace. *)
+    valid_state_console : valid_console st.(st_trace);
+    (* The console buffer never overflows *)
+    valid_state_console_len : valid_console_len st.(st_trace);
+  }.
+
+  Lemma hd_error_app {A} : forall (xs ys : list A) x,
+    hd_error xs = Some x ->
+    hd_error (xs ++ ys) = Some x.
+  Proof.
+    destruct xs; cbn; easy.
+  Qed.
+
+  Lemma compute_console_ridx_increase : forall tr ev ridx c ridx' c',
+    let cons := compute_console tr in
+    let cons' := compute_console (ev :: tr) in
+    valid_console (ev :: tr) ->
+    valid_trace_serial (ev :: tr) ->
+    hd_error cons = Some (c, ridx) ->
+    hd_error cons' = Some (c', ridx') ->
+    (ridx <= ridx')%nat.
+  Proof.
+    destruct ev; intros * Hcons Htr Hhd Hhd'; red in Hcons, Htr; subst cons cons'; cbn in *.
+    - destruct (_ <? _)eqn:Hlt; [rewrite Z.ltb_lt in Hlt | rewrite Z.ltb_nlt in Hlt].
+      + erewrite hd_error_app in Hhd' by eauto; inj; auto.
+      + pose proof console_len_pos.
+        destruct (compute_console tr) eqn:Heq; cbn in *; inj; try lia.
+        admit.
+    - admit.
+    - admit.
+  Admitted.
+
+  (* Lemma compute_console_ridx_increase : forall ridx c tr ridx' c', *)
+  (*   let cons := compute_console tr in *)
+  (*   let cons' := compute_console (ETReadUser ridx c :: tr) in *)
+  (*   hd_error cons = Some (c', ridx') -> *)
+  (*   (ridx' < ridx)%nat. *)
+  (* Proof. *)
+  (*   induction tr as [| ev tr]; cbn; intros * Hhd; [discriminate |]. *)
+  (*   destruct ev; eauto. *)
+  (*   - admit. *)
+  (*   - eapply IHtr. *)
+  (* Qed. *)
+
+  Lemma serial_getc_preserve_trace_unique : forall st st',
+    valid_state st ->
     serial_getc st = st' ->
-    valid_trace st'.
+    valid_trace_unique st'.(st_trace).
   Proof.
-    unfold valid_trace, serial_getc; intros * Hvalid Hspec c Hin.
-    destruct st as [? ? tr]; inv Hspec; cbn in *.
-    rewrite in_app_iff in Hin; cbn in Hin.
-    intuition.
-    inv H0; eauto.
+    unfold serial_getc; intros * Hvalid Hspec.
+    destruct st as [? tr]; subst; destruct Hvalid; cbn in *.
+    constructor; auto.
+    intros * Hin.
+    apply valid_state_trace_serial0 in Hin.
+    destruct Hin as (? & ? & Hlen & ? & Hsub); cbn in Hsub.
+    rewrite Z.max_l in Hsub
+      by (rewrite !Zlength_correct, Hlen; lia).
+    rewrite conclib.sublist_all in Hsub by easy.
+    rewrite Hsub in Hlen; cbn in Hlen; lia.
   Qed.
 
-  Lemma serial_getc_preserve_valid_console : forall st st',
-    valid_console st ->
+  Lemma serial_getc_preserve_valid_state : forall st st',
+    valid_state st ->
     serial_getc st = st' ->
-    valid_console st'.
+    valid_state st'.
   Proof.
-    unfold valid_console, serial_getc; intros * (Hlen & Hvalid) Hspec.
-    destruct st as [? cons ?]; inv Hspec; cbn in *.
-    rewrite ?Zlength_correct in *.
-    destruct (_ <? _) eqn:Hlt; [rewrite Z.ltb_lt in Hlt | rewrite Z.ltb_nlt in Hlt].
-    + rewrite app_length; cbn.
-      split; try lia.
-      intros c; rewrite ?in_app_iff; cbn.
-      intuition (subst; auto).
-    + pose proof console_len_pos.
-      rewrite app_length; cbn.
-      split; [destruct cons; cbn in *; lia |].
-      intros c; rewrite ?in_app_iff; cbn.
-      destruct cons; intuition (subst; auto).
-      intuition.
+    unfold serial_getc; intros * Hvalid Hspec.
+    pose proof Hvalid as Hvalid'.
+    eapply serial_getc_preserve_trace_unique in Hvalid'; eauto.
+    destruct st as [? tr]; subst; destruct Hvalid; cbn in *.
+    split; cbn; red; auto.
+    - (* valid_trace_serial *)
+      rewrite !Zlength_cons.
+      intros *; cbn.
+      intuition eauto; inj.
+      + repeat (esplit; eauto); try lia.
+        rewrite Z.max_l by lia.
+        rewrite conclib.sublist_all; auto.
+        rewrite Zlength_cons; easy.
+      + edestruct valid_state_trace_serial0 as (tr' & ? & ? & ? & Hsub); eauto; subst.
+        repeat (esplit; eauto); try lia.
+        rewrite <- Hsub.
+        rewrite Z.max_r by lia.
+        apply Z.max_case_strong; intros.
+        * (* length tr <= length tr' + 1 *)
+          rewrite Z.max_l in Hsub by lia; cbn in Hsub.
+          rewrite conclib.sublist_all in Hsub by lia; subst.
+          rewrite ?Zlength_cons in *.
+          replace (Z.succ _ - (_ + 1)) with 1 by lia.
+          rewrite conclib.sublist_S_cons by lia.
+          f_equal; lia.
+        * (* length tr' + 1 <= length tr *)
+          rewrite Z.max_r in Hsub by lia; cbn in Hsub.
+          rewrite conclib.sublist_S_cons by lia.
+          f_equal; lia.
+    - (* valid_trace_user *)
+      intros * Heq.
+      pose proof Heq as Heq'.
+      apply list_eq_in_r in Heq'; try congruence.
+      apply in_split in Heq'.
+      destruct Heq' as (post' & pre' & ?); subst.
+      rewrite app_comm_cons in Heq.
+      apply list_unique_match in Heq; auto.
+      destruct Heq as (? & ?); subst; eauto.
+    - (* valid_console *)
+      intros *; cbn.
+      rewrite !in_app_iff, Zlength_correct; cbn.
+      destruct (_ <? _) eqn:Hlt; [rewrite Z.ltb_lt in Hlt | rewrite Z.ltb_nlt in Hlt].
+      + intuition (inj; auto).
+      + red in valid_state_console0.
+        destruct (compute_console tr); intuition (inj; auto; try easy).
+        intuition.
+    - (* valid_console_len *)
+      red in valid_state_console_len0.
+      repeat (rewrite ?Zlength_correct, ?app_length in *; cbn).
+      pose proof console_len_pos.
+      destruct (_ <? _) eqn:Hlt; [rewrite Z.ltb_lt in Hlt | rewrite Z.ltb_nlt in Hlt];
+        try lia.
+      destruct (compute_console tr); cbn in *; lia.
   Qed.
 
-  Lemma getchar_spec_preserve_valid_trace : forall st st' c tr,
-    valid_trace st ->
-    getchar_spec st = (st', c, tr) ->
-    valid_trace st'.
+  Lemma console_read_preserve_trace_unique : forall st st' c,
+    valid_state st ->
+    console_read st = (st', c) ->
+    valid_trace_unique st'.(st_trace).
   Proof.
-    unfold valid_trace, getchar_spec, console_read; intros * Hvalid Hspec c Hin.
-    destruct st as [? [| c' cons] ?].
-    - inv Hspec; eauto.
-    - destruct (0 <=? c'); inv Hspec; cbn in *; eauto.
-  Qed.
+    unfold console_read; intros * Hvalid Hspec.
+    destruct st as [? tr]; destruct Hvalid; cbn in *.
+    destruct (compute_console tr) as [| (c' & ridx) cons] eqn:Hcons; inj; red; cbn; auto.
+    constructor; auto.
+    intros Hin; apply in_split in Hin.
+    destruct Hin as (post & pre & ?); subst.
+    edestruct valid_state_trace_user0 as (Hin & Hhd); eauto.
+    admit.
+  Admitted.
 
-  Lemma getchar_spec_preserve_valid_console : forall st st' c tr,
-    valid_console st ->
-    getchar_spec st = (st', c, tr) ->
-    valid_console st'.
+  Definition new_trace (st st' : state) : etrace :=
+    snd (split_at_common_prefix IO_trace_event_eq st.(st_trace) st'.(st_trace)).
+
+  Definition valid_ret (st st' : state) (c : Z) :=
+    (c = -1 \/ 0 <= c <= 255) /\ st.(st_mem) = st'.(st_mem) /\
+    (c = -1 -> new_trace st st' = nil) /\
+    (0 <= c <= 255 -> exists ridx, new_trace st st' = ETReadUser ridx c :: nil).
+
+  Lemma console_read_preserve_valid_state : forall st st' c,
+    valid_state st ->
+    console_read st = (st', c) ->
+    valid_state st' /\ valid_ret st st' c.
   Proof.
-    unfold valid_console, getchar_spec, console_read; intros * (Hlen & Hvalid) Hspec.
-    destruct st as [? [| c' cons] ?].
-    - inv Hspec; eauto.
-    - rewrite ?Zlength_correct in *.
-      destruct (0 <=? c'); inv Hspec; cbn in *; split; eauto; lia.
+    admit.
+  (*   unfold console_read; intros * Hvalid Hspec. *)
+  (*   destruct st as [? [| (c' & ridx) cons] tr]; destruct Hvalid; inj; cbn in *. *)
+  (*   { repeat (split; eauto). } *)
+  (*   split; [split; red |]; rewrite ?Zlength_correct in *; cbn -[Z.of_nat] in *; *)
+  (*     eauto; try lia. *)
+  (*   - (1* valid_trace_serial *1) *)
+  (*     intros *; rewrite in_app_iff; cbn. *)
+  (*     intuition (try congruence). *)
+  (*     edestruct valid_state_trace_serial0 as (tr' & ? & ? & Hsub); eauto; subst. *)
+  (*     repeat (esplit; eauto). *)
+  (*     rewrite sublist0_app1; auto. *)
+  (*     replace (Zlength tr' + 1) *)
+  (*       with (Zlength (tr' ++ ETReadOS (length tr') (serial_oracle tr') :: nil)) *)
+  (*       by (rewrite Zlength_app; auto). *)
+  (*     rewrite <- Hsub. *)
+  (*     auto using conclib.sublist_max_length, Zlength_nonneg. *)
+  (*   - (1* valid_trace_user *1) *)
+  (*     intros ridx' c' * Heq. *)
+  (*     assert (Hcase: ETReadUser ridx c = ETReadUser ridx' c' \/ *)
+  (*                    ETReadUser ridx c <> ETReadUser ridx' c'). *)
+  (*     { clear; repeat decide equality. } *)
+  (*     destruct Hcase; inj. *)
+  (*     + apply list_unique_match in Heq; auto. *)
+  (*       { destruct Heq; subst; auto. *)
+  (*         split. *)
+  (*         - eapply valid_state_console0; cbn; auto. *)
+  (*         - hnf in *. *)
+  (*       } *)
+  (*       apply conclib.NoDup_add; rewrite app_nil_r; auto. *)
+  (*       intros Hin. *)
+  (*       apply in_split in Hin. *)
+  (*       destruct Hin as (pre' & post' & ?); subst. *)
+  (*       assert (Hin: In (ETReadOS ridx' c') (pre' ++ ETReadUser ridx' c' :: post')). *)
+  (*       { rewrite in_app_iff; left. *)
+  (*         eapply valid_state_trace_user0; eauto. } *)
+  (*       eapply valid_state_trace_serial0 in Hin. *)
+  (*       destruct Hin as (? & ? & ? & ?); subst. *)
+  (*       red in valid_state_console0. *)
+  (*     + pose proof Heq as Heq'. *)
+  (*       apply list_eq_in_l in Heq'; auto. *)
+  (*       apply in_split in Heq'. *)
+  (*       destruct Heq' as (pre' & post' & Heq''). *)
+  (*       assert (In (ETReadOS ridx' c') pre'). *)
+  (*       { apply valid_state_trace_user0 in Heq''; auto. } *)
+  (*       subst. *)
+  (*   - (1* valid_console *1) *)
+  (*     intuition idtac. *)
+  (*   - (1* c in range *1) *)
+  (*     pose proof serial_oracle_in_range. *)
+  (*     right; cut (exists tr, serial_oracle tr = c); eauto. *)
+  (*     intros (? & ?); subst; eauto. *)
+  Admitted.
+
+  Lemma getchar_spec_preserve_valid_state : forall st st' c,
+    valid_state st ->
+    getchar_spec st = (st', c) ->
+    valid_state st' /\ valid_ret st st' c.
+  Proof.
+    unfold getchar_spec; intros * Hvalid Hspec.
+    destruct (console_read st) eqn:Hread.
+    eapply console_read_preserve_valid_state in Hread; eauto.
+    destruct (0 <=? _) eqn:Hle; inj; eauto.
+    rewrite Z.leb_nle in Hle.
+    destruct Hread as (? & ([? | ?] & ? & ? & ?)); subst; try lia.
+    repeat (split; auto).
   Qed.
 
 End Specs.
@@ -233,46 +535,43 @@ Section SpecsCorrect.
       is_trace z t' ->
       is_trace z0 (app_trace t t').
 
-  Lemma getchar_correct k z m c t :
+  Lemma getchar_correct k z st :
     (* Initial state is valid *)
-    let st := mkSt m c t in
     valid_state st ->
     (* Pre condition holds *)
-    getchar_pre' m k z ->
-    exists st' r t',
+    getchar_pre' st.(st_mem) k z ->
+    exists st' r,
       (* Spec with same initial memory returns some state and result *)
-      getchar_spec st = (st', r, t') /\
+      getchar_spec st = (st', r) /\
+      (* Compute the newly added events *)
+      let t' := new_trace st st' in
       (* New itree is old k applied to result, or same as old itree if nothing
          to read *)
       let z' := if 0 <=? r then k (Int.repr r) else z in
       (* Post condition holds on new state, itree, and result *)
-      getchar_post' m st'.(st_mem) (Int.repr r) (k, z) z' /\
+      getchar_post' st.(st_mem) st'.(st_mem) (Int.repr r) (k, z) z' /\
       (* The new itree 'consumed' the generated trace *)
       consume_trace z z' t'.
   Proof.
     unfold getchar_pre'; intros Hval Hpre; cbn.
-    unfold getchar_spec; cbn.
-    destruct c as [| r c]; cbn.
-    - (* Nothing to read *)
-      do 4 esplit; eauto.
-      split; hnf; cbn; auto.
-    - (* Read r *)
-      destruct Hval as (Hval_tr & (Hlen & Hval_cons)).
-      specialize (Hval_cons _ ltac:(cbn; auto)).
-      specialize (Hval_tr _ Hval_cons).
-      destruct Hval_tr as (? & Hr).
-      assert (0 <= r <= 255)
-        by (subst; apply serial_oracle_in_range; auto).
+    destruct (getchar_spec st) as (st' & r) eqn:Hspec.
+    eapply getchar_spec_preserve_valid_state in Hspec; auto.
+    destruct Hspec as (Hval' & (Hr & Hmem & Htr & Htr')).
+    exists st', r.
+    repeat (split; auto).
+    - destruct Hr; subst; auto.
+      rewrite Int.signed_repr by (cbn; lia).
       rewrite Zle_imp_le_bool by lia.
-      do 4 esplit; eauto.
-      rewrite Zle_imp_le_bool by lia.
-      split; hnf; cbn.
-      + rewrite Int.signed_repr; auto.
-        cbn; lia.
-      + intros * Htrace.
+      auto.
+    - hnf; intros * Htrace.
+      (* apply Hpre. *)
+      destruct Hr; subst; cbn in *.
+      + rewrite Htr; auto.
+      + destruct Htr' as (? & ->); auto.
         apply Hpre.
         hnf; cbn.
         repeat constructor.
+        rewrite Zle_imp_le_bool in Htrace by lia.
         apply Htrace.
   Qed.
 
